Flapjack/Tests.lean
@@ -64,6 +64,7 @@ import Flapjack.Test.StaticRedecVarParity
 import Flapjack.Test.StaticExportParamsParity
 import Flapjack.Test.StaticOperandsParity
 import Flapjack.Test.StaticFuncArgsParity
+import Flapjack.Test.StaticStructFieldsParity
 import Flapjack.Test.CorrectnessConditional
 import Flapjack.Test.CorrectnessColour
 import Flapjack.Test.CorrectnessSsaColour
